common/Assoc.v
@@ -1,0 +1,205 @@
+Require Import Coqlib List.
+
+Section ASSOC.
+  Variables A B: Type.
+
+  Variable Aeq: forall (a1 a2: A), {a1=a2}+{a1<>a2}.
+
+  Fixpoint get_assoc (l: list (A*B)) (b: A) : option B :=
+    match l with
+      nil => None
+    | (k,v)::r => if Aeq k b then Some v else get_assoc r b
+    end.
+
+  Lemma get_assoc_in_fst:
+    forall (l: list (A*B)) b r,
+      get_assoc l b = Some r ->
+      In b (map fst l).
+  Proof.
+    induction l; simpl; intros; eauto. inv H.
+    repeat destr_in H. simpl. right.
+    eauto.
+  Qed.
+
+  Lemma get_assoc_in:
+    forall (l: list (A*B)) b r,
+      get_assoc l b = Some r ->
+      In (b,r) l.
+  Proof.
+    induction l; simpl; intros; eauto. inv H.
+    repeat destr_in H. simpl. right.
+    eauto.
+  Qed.
+
+  Lemma in_lnr_get_assoc:
+    forall l b f,
+      list_norepet (map fst l) ->
+      In (b,f) l ->
+      get_assoc l b = Some f.
+  Proof.
+    induction l; intros b f LNR IN; simpl in *. easy.
+    destruct IN. subst. destr.
+    inv LNR. erewrite IHl; eauto.
+    repeat destr. subst. simpl in *.
+    exfalso; apply H2; apply in_map_iff.
+    exists (b,f); split; auto.
+  Qed.
+
+End ASSOC.
+
+
+(* 
+
+Fixpoint range_Z (o: Z) (n: nat) : list Z :=
+  match n with
+    O => nil
+  | Datatypes.S m => o :: range_Z (o+1) m
+  end.
+
+Definition range_eqb (o size: Z) (f: Z -> bool) : bool:=
+  forallb f (range_Z o (Z.to_nat size)).
+
+
+Lemma in_range_Z:
+  forall n s o,
+    In o (range_Z s n) ->
+    s <= o < s + Z.of_nat n.
+Proof.
+  induction n; intros. easy.
+  destruct H. subst. simpl. generalize (Pos2Z.is_pos (Pos.of_succ_nat n)). omega.
+  apply IHn in H. split. omega. rewrite Nat2Z.inj_succ. omega.
+Qed.
+
+Lemma range_eqb_forall:
+  forall lo s f,
+    (forall o, lo <= o < lo + s -> f o = true) ->
+    0 <= s ->
+    range_eqb lo s f = true.
+Proof.
+  unfold range_eqb. intros lo s f H POS.
+  rewrite forallb_forall. intros.
+  apply in_range_Z in H0.
+  apply H. rewrite Z2Nat.id in H0. omega.  auto.
+Qed.
+
+Lemma range_eqb_and:
+  forall lo1 lo2 s1 s2 f,
+    0 <= s1 -> 0 <= s2 ->
+    (forall o, lo1 <= o < lo1 + s1 \/ lo2 <= o < lo2 + s2 -> f o = true) ->
+    range_eqb lo1 s1 f = true /\
+    range_eqb lo2 s2 f = true.
+Proof.
+  intros.
+  rewrite ! range_eqb_forall; auto.
+Qed.
+
+Definition disjointb lo1 n1 lo2 n2 : bool :=
+  range_eqb lo1 n1 (fun o1 => range_eqb lo2 n2 (fun o2 => negb (Z.eqb o1 o2))).
+
+Lemma in_range_Z':
+  forall n s o,
+    s <= o < s + Z.of_nat n ->
+    In o (range_Z s n).
+Proof.
+  induction n; intros. simpl in H. omega.
+  simpl in *.
+  destruct (zeq s o); auto.
+  right. apply IHn. split. omega.
+  rewrite Zpos_P_of_succ_nat in H. omega.
+Qed.
+
+Lemma range_eqb_forall':
+  forall lo s f,
+    0 <= s ->
+    range_eqb lo s f = true ->
+    (forall o, lo <= o < lo + s -> f o = true).
+Proof.
+  unfold range_eqb. intros lo s f POS RE.
+  rewrite forallb_forall in RE. intros.
+  apply RE.
+  apply in_range_Z'.
+  rewrite Z2Nat.id. omega.  auto.
+Qed.
+
+Lemma disjointb_disjoint:
+  forall lo1 n1 lo2 n2,
+    disjointb lo1 n1 lo2 n2 = true ->
+    forall o,
+      lo1 <= o < lo1 + n1 ->
+      lo2 <= o < lo2 + n2 ->
+      False.
+Proof.
+  intros lo1 n1 lo2 n2 DISJ o IN1 IN2.
+  unfold disjointb in DISJ.
+  eapply range_eqb_forall' in DISJ; eauto.
+  2: omega.
+  eapply range_eqb_forall' in DISJ; eauto.
+  2: omega.
+  apply negb_true_iff in DISJ.
+  apply Z.eqb_neq in DISJ. congruence.
+Qed.
+
+Lemma disjoint_disjointb:
+  forall lo1 n1 lo2 n2,
+  (forall o,
+      lo1 <= o < lo1 + n1 ->
+      lo2 <= o < lo2 + n2 ->
+      False) ->
+  0 <= n1 ->
+  0 <= n2 ->
+  disjointb lo1 n1 lo2 n2 = true .
+Proof.
+  intros lo1 n1 lo2 n2 DISJ P1 P2.
+  unfold disjointb.
+  eapply range_eqb_forall; eauto.
+  intros.
+  eapply range_eqb_forall; eauto.
+  intros.
+  apply negb_true_iff.
+  apply Z.eqb_neq. intro; subst. eapply DISJ; eauto.
+Qed.
+
+
+
+  Definition inject_option_frame delta fi fi' :=
+    match fi, fi' with
+      None, None => True
+    | Some fi, Some fi' => inject_frame_info delta fi fi'
+    | _,_ => False
+    end.
+
+  Lemma inject_option_frame_id:
+    forall o,
+      inject_option_frame 0 o o.
+  Proof.
+    unfold inject_option_frame.
+    destruct o; auto.
+  Qed.
+
+  Hint Resolve inject_option_frame_id.
+
+  Lemma inject_option_frame_trans:
+    forall o1 o2 o3 delta1 delta2,
+      inject_option_frame delta1 o1 o2 ->
+      inject_option_frame delta2 o2 o3 ->
+      inject_option_frame (delta1 + delta2) o1 o3.
+  Proof.
+    unfold inject_option_frame.
+    intros o1 o2 o3 delta1 delta2 A B.
+    destruct o1, o2, o3; eauto; easy.
+  Qed.
+
+  Hint Resolve inject_option_frame_trans.
+
+  Lemma inject_option_frame_inv:
+    forall z ofi fi,
+      inject_option_frame z ofi (Some fi) ->
+      exists f, ofi = Some f /\ inject_frame_info z f fi.
+  Proof.
+    intros. 
+    destruct ofi; simpl in H; try easy.
+    eauto. 
+  Qed.
+
+
+ *)
